@prefix bio: <https://bioschemas.org/> .
@prefix dcterms: <http://purl.org/dc/terms/> .
@prefix dmib: <https://biomedit.ch/rdf/sphn-schema/dmib#> .
@prefix foaf: <http://xmlns.com/foaf/0.1/> .
@prefix imag: <https://imaging-plaza.epfl.ch/ontology#> .
@prefix md4i: <http://w3id.org/nfdi4ing/metadata4ing#> .
@prefix owl: <http://www.w3.org/2002/07/owl#> .
@prefix qb: <http://purl.org/linked-data/cube#> .
@prefix rdf: <http://www.w3.org/1999/02/22-rdf-syntax-ns#> .
@prefix rdfs: <http://www.w3.org/2000/01/rdf-schema#> .
@prefix schema: <http://schema.org/> .
@prefix sd: <https://w3id.org/okn/o/sd#> .
@prefix sh: <http://www.w3.org/ns/shacl#> .
@prefix skos: <http://www.w3.org/2004/02/skos/core#> .
@prefix sphn: <https://biomedit.ch/rdf/sphn-schema/sphn#> .
@prefix vann: <http://purl.org/vocab/vann/> .
@prefix xsd: <http://www.w3.org/2001/XMLSchema#> .

schema:ComputerLanguage a rdfs:Class ;
    rdfs:label "Computer language" ;
    rdfs:comment "This type covers computer programming languages such as Scheme and Lisp, as well as other language-like computer representations. Natural languages are best represented with the Language type." ;
    rdfs:subClassOf schema:Intangible .

schema:DataFeed a rdfs:Class,
        sh:NodeShape ;
    rdfs:label "Data feed" ;
    rdfs:comment "A single feed providing structured information about one or more entities or topics." ;
    rdfs:subClassOf schema:Dataset ;
    sh:property schema:DataDownload-contentURL,
        schema:Dataset-measurementTechnique,
        schema:Dataset-variableMeasured,
        schema:Thing-description,
        schema:Thing-name,
        imag:SoftwareApplication-imagingModalityShape,
        imag:bodySiteShape,
        imag:datasetFormatShape,
        imag:hasPhysicalQuantityShape,
        imag:resolutionShape,
        sd:DatasetSpecification-hasDimensionality .

schema:Grant a rdfs:Class ;
    rdfs:label "Grant" ;
    rdfs:comment "A grant, typically financial or otherwise quantifiable, of resources." ;
    rdfs:subClassOf schema:Intangible .

schema:Organization a rdfs:Class,
        sh:NodeShape ;
    rdfs:label "Organization" ;
    rdfs:comment "An organization such as a school, NGO, corporation, club, etc." ;
    rdfs:subClassOf schema:Thing ;
    sh:property schema:Organization-legalName,
        md4i:hasRorIdShape .

schema:Person a rdfs:Class,
        sh:NodeShape ;
    rdfs:label "Person" ;
    rdfs:comment "A person (alive, dead, undead, or fictional)." ;
    rdfs:subClassOf schema:Thing ;
    owl:equivalentClass foaf:Person ;
    sh:property schema:Person-affiliation,
        schema:Thing-name,
        md4i:orcidIdShape .

schema:SoftwareSourceCode a rdfs:Class,
        sh:NodeShape ;
    rdfs:label "Software application" ;
    rdfs:comment "A software application." ;
    rdfs:subClassOf schema:CreativeWork ;
    sh:property schema:CreativeWork-author,
        schema:CreativeWork-citation,
        schema:CreativeWork-conditionsOfAccess,
        schema:CreativeWork-dateCreated,
        schema:CreativeWork-datePublished,
        schema:CreativeWork-isAccessibleForFree,
        schema:CreativeWork-isBasedOn,
        schema:CreativeWork-license,
        schema:SoftwareApplication-applicationCategory,
        schema:SoftwareApplication-featureList,
        schema:SoftwareApplication-memoryRequirements,
        schema:SoftwareApplication-operatingSystem,
        schema:SoftwareApplication-processorRequirements,
        schema:SoftwareApplication-softwareRequirements,
        schema:SoftwareApplication-supportingData,
        schema:SoftwareSourceCode-codeRepository,
        schema:SoftwareSourceCode-programmingLanguage,
        schema:Thing-description,
        schema:Thing-identifier,
        schema:Thing-image,
        schema:Thing-name,
        schema:Thing-url,
        imag:SoftwareApplication-hasExecutableNotebook,
        imag:SoftwareApplication-imagingModalityShape,
        imag:SoftwareApplication-requiresGPUShape,
        imag:SoftwareApplication-runnableExampleShape,
        imag:fairLevelShape,
        imag:isPluginModuleOfShape,
        imag:relatedToOrganizationShape,
        sd:SoftwareApplication-hasAcknowledgements,
        sd:SoftwareApplication-hasDocumentation,
        sd:SoftwareApplication-hasExecutableInstructions,
        sd:SoftwareApplication-hasFunding,
        sd:SoftwareApplication-hasParameter,
        sd:SoftwareApplication-readme,
        sd:SoftwareConfiguration-hasSoftwareImage ;
    sh:rule [ a sh:TripleRule ;
            sh:condition imag:fairlevel0Shape ;
            sh:object "Fair level 0" ;
            sh:predicate imag:fairLevel ;
            sh:subject sh:this ],
        [ a sh:TripleRule ;
            sh:condition imag:fairlevel1Shape ;
            sh:object "Fair level 1" ;
            sh:predicate imag:fairLevel ;
            sh:subject sh:this ],
        [ a sh:TripleRule ;
            sh:condition imag:fairlevel2Shape ;
            sh:object "Fair level 2" ;
            sh:predicate imag:fairLevel ;
            sh:subject sh:this ],
        [ a sh:TripleRule ;
            sh:condition imag:fairlevel3Shape ;
            sh:object "Fair level 3" ;
            sh:predicate imag:fairLevel ;
            sh:subject sh:this ],
        [ a sh:TripleRule ;
            sh:condition imag:fairlevel4Shape ;
            sh:object "Fair level 4" ;
            sh:predicate imag:fairLevel ;
            sh:subject sh:this ],
        [ a sh:TripleRule ;
            sh:condition imag:fairlevel5Shape ;
            sh:object "Fair level 5" ;
            sh:predicate imag:fairLevel ;
            sh:subject sh:this ],
        imag:FeatureTaggerRule .

bio:FormalParameter a rdfs:Class,
        sh:NodeShape ;
    rdfs:label "Formal Parameter"@en ;
    rdfs:comment "A FormalParameter is an identified variable used to stand for the actual value(s) that are consumed/produced by a set of steps"@en ;
    rdfs:subClassOf qb:DataStructureDefinition ;
    sh:property schema:CreativeWork-encodingFormat,
        schema:PropertyValueSpecification-defaultValue,
        schema:PropertyValueSpecification-valueRequired,
        schema:Thing-description,
        schema:Thing-name,
        sd:DatasetSpecification-hasDimensionality,
        sd:DatasetSpecification-hasFormat .

imag:AffiliationEnum a rdfs:Class ;
    rdfs:label "Affiliation Enumeration" ;
    rdfs:comment "Enumeration class for affiliation" ;
    rdfs:subClassOf imag:EnumerationType .

imag:ApplicationCategoryEnum a rdfs:Class ;
    rdfs:label "Application Category Enumeration" ;
    rdfs:comment "Enumeration class for application category" ;
    rdfs:subClassOf imag:EnumerationType .

imag:ComputerLanguageEnum a rdfs:Class ;
    rdfs:label "Computer Language Enumeration" ;
    rdfs:comment "Enumeration class for computer languages" ;
    rdfs:subClassOf imag:EnumerationType .

imag:DatasetFormatEnumeration a rdfs:Class ;
    rdfs:label "Dataset Format Enumeration" ;
    rdfs:comment "Enumeration class for dataset formats" ;
    rdfs:subClassOf imag:EnumerationType .

imag:EnumerationType a rdfs:Class ;
    rdfs:label "Enumeration Type" ;
    rdfs:comment "EnumerationType class used to group all enumeration classes under" ;
    rdfs:subClassOf schema:Enumeration .

imag:ExecutableNotebook a rdfs:Class,
        sh:NodeShape ;
    rdfs:label "Executable Notebook"@en ;
    rdfs:comment "An object representing an executable notebook such as Jupyter Notebook" ;
    sh:property schema:Thing-description,
        schema:Thing-name,
        schema:Thing-url .

imag:FeatureEnum a rdfs:Class ;
    rdfs:label "Feature Enumeration" ;
    rdfs:comment "Enumeration class for software features" ;
    rdfs:subClassOf imag:EnumerationType .

imag:HostTypeEnumeration a rdfs:Class ;
    rdfs:label "Host Type Enumeration" ;
    rdfs:comment "Enumeration class for host type" ;
    rdfs:subClassOf imag:EnumerationType .

imag:ImageObject a rdfs:Class ;
    rdfs:label "Image object" ;
    rdfs:comment "An image of the software, typically a screenshot, before/after or a logo." ;
    rdfs:subClassOf schema:Intangible .

imag:ImageObjectTagEnum a rdfs:Class ;
    rdfs:label "Image Object Tag Enumeration" ;
    rdfs:comment "Enumeration class for image object tag" ;
    rdfs:subClassOf imag:EnumerationType .

imag:ImagingModalityEnum a rdfs:Class ;
    rdfs:label "Imaging Modality Enumeration" ;
    rdfs:comment "Enumeration class for imaging modality" ;
    rdfs:subClassOf imag:EnumerationType .

imag:IsPluginModuleOfEnum a rdfs:Class ;
    rdfs:label "Plugin Module Enumeration" ;
    rdfs:comment "Enumeration class for plugin module" ;
    rdfs:subClassOf imag:EnumerationType .

imag:OperatingSystemEnum a rdfs:Class ;
    rdfs:label "Operating System Enumeration" ;
    rdfs:comment "Enumeration class for operating system" ;
    rdfs:subClassOf imag:EnumerationType .

imag:ProcessorRequirementsEnum a rdfs:Class ;
    rdfs:label "Processor Requirements Enumeration" ;
    rdfs:comment "Enumeration class for processor requirements" ;
    rdfs:subClassOf imag:EnumerationType .

imag:RunnableExample a rdfs:Class,
        sh:NodeShape ;
    rdfs:label "Runnable example" ;
    rdfs:comment "A runnable example of the software component"@en ;
    sh:property schema:Thing-description,
        schema:Thing-name,
        schema:Thing-url,
        imag:hostTypeShape .

imag:SoftwareRequirementsEnum a rdfs:Class ;
    rdfs:label "Software Requirements Enumeration" ;
    rdfs:comment "Enumeration class for software requirements" ;
    rdfs:subClassOf imag:EnumerationType .

sd:DatasetSpecification a rdfs:Class ;
    rdfs:label "Dataset Specification"@en ;
    rdfs:comment "Class designed to describe a type of input or output used or produced by a model. For example, Topoflow has several inputs. One of them is a text file with precipitation values. The representation of this input is an instance of a dataset specification."@en ;
    rdfs:subClassOf qb:DataStructureDefinition .

sd:FundingInformation a rdfs:Class,
        sh:NodeShape ;
    rdfs:label "Funding Information"@en ;
    rdfs:comment "A class to represent the funding information of a software project"@en ;
    sh:property schema:Thing-identifier,
        sd:FundingInformation-fundingGrant,
        sd:FundingInformation-fundingSource .

sd:SoftwareImage a rdfs:Class,
        sh:NodeShape ;
    rdfs:label "Software Image"@en ;
    rdfs:comment "An image that virtualizes the functionality of a given software. For example, a Docker container."@en ;
    rdfs:subClassOf sd:Software ;
    sh:property schema:SoftwareApplication-softwareVersion,
        schema:Thing-description,
        schema:Thing-name,
        sd:SoftwareImage-availableInRegistry .

schema:Person-familyName a sh:PropertyShape ;
    sh:datatype xsd:string ;
    sh:minCount 1 ;
    sh:path schema:familyName .

schema:Person-givenName a sh:PropertyShape ;
    sh:datatype xsd:string ;
    sh:minCount 1 ;
    sh:path schema:givenName .

schema:distribution a rdf:Property ;
    rdfs:label "Distribution" ;
    rdfs:comment "A downloadable form of this dataset, at a specific location, in a specific format." .

imag:AMD64 a imag:ProcessorRequirementsEnum ;
    rdfs:label "AMD64" .

imag:ARM64 a imag:ProcessorRequirementsEnum ;
    rdfs:label "ARM64" .

imag:AfterImage a imag:ImageObjectTagEnum ;
    rdfs:label "after image" .

imag:AnimatedImage a imag:ImageObjectTagEnum ;
    rdfs:label "animated image" .

imag:Any a imag:ImagingModalityEnum ;
    rdfs:label "Any" .

imag:Bash a imag:ComputerLanguageEnum ;
    rdfs:label "bash" .

imag:BeforeImage a imag:ImageObjectTagEnum ;
    rdfs:label "before image" .

imag:C a imag:ComputerLanguageEnum ;
    rdfs:label "C" .

imag:CAT a imag:ImagingModalityEnum ;
    rdfs:label "CAT" .

imag:CSV_TSV a imag:DatasetFormatEnumeration ;
    rdfs:label "CSV/TSV (Tabular Data)" .

imag:CUDA_10_1 a imag:SoftwareRequirementsEnum ;
    rdfs:label "CUDA 10.1" .

imag:CUDA_11_8 a imag:SoftwareRequirementsEnum ;
    rdfs:label "CUDA 11.8" .

imag:CUDA_12_1 a imag:SoftwareRequirementsEnum ;
    rdfs:label "CUDA 12.1" .

imag:CUDA_9_0 a imag:SoftwareRequirementsEnum ;
    rdfs:label "CUDA 9.0" .

imag:Classification a imag:FeatureEnum ;
    rdfs:label "Classification" ;
    skos:broader imag:Segmentation .

imag:Clustering a imag:FeatureEnum ;
    rdfs:label "Clustering" ;
    skos:broader imag:Segmentation .

imag:Cplusplus a imag:ComputerLanguageEnum ;
    rdfs:label "C++" .

imag:Csharp a imag:ComputerLanguageEnum ;
    rdfs:label "C#" .

imag:CurvatureEstimation a imag:FeatureEnum ;
    rdfs:label "Curvature estimation" ;
    skos:broader imag:SceneReconstruction .

imag:DICOM a imag:DatasetFormatEnumeration ;
    rdfs:label "DICOM (Medical Imaging Format)" .

imag:Deblurring a imag:FeatureEnum ;
    rdfs:label "Deblurring" ;
    skos:broader imag:Denoising .

imag:Deconvolution a imag:FeatureEnum ;
    rdfs:label "Deconvolution" ;
    skos:broader imag:Denoising .

imag:DepthEstimation a imag:FeatureEnum ;
    rdfs:label "Depth estimation" ;
    skos:broader imag:SceneReconstruction .

imag:DesktopApp a imag:ApplicationCategoryEnum ;
    rdfs:label "Desktop app" .

imag:DigitalImageCorrelation a imag:FeatureEnum ;
    rdfs:label "Digital image correlation" ;
    skos:broader imag:OpticalFlow .

imag:DimensionalityReduction a imag:FeatureEnum ;
    rdfs:label "Dimensionality reduction" ;
    skos:broader imag:FeatureExtraction .

imag:DirectionalImageAnalysis a imag:FeatureEnum ;
    rdfs:label "Directional image analysis" ;
    skos:broader imag:FeatureExtraction .

imag:DistributionMeasurements a imag:FeatureEnum ;
    rdfs:label "Distribution measurements" ;
    skos:broader imag:StatisticsMeasurement .

imag:DriftCorrection a imag:FeatureEnum ;
    rdfs:label "Drift correction" ;
    skos:broader imag:OpticalFlow .

imag:EPFL a imag:AffiliationEnum ;
    rdfs:label "EPFL" .

imag:ETHZ a imag:AffiliationEnum ;
    rdfs:label "ETHZ" .

imag:FeatureDetection a imag:FeatureEnum ;
    rdfs:label "Feature detection" ;
    skos:broader imag:MorphologicalAnalysis .

imag:Fiji a imag:IsPluginModuleOfEnum ;
    rdfs:label "Fiji" .

imag:Filtering a imag:FeatureEnum ;
    rdfs:label "Filtering" ;
    skos:broader imag:Preprocessing .

imag:GoLang a imag:ComputerLanguageEnum ;
    rdfs:label "GoLang" .

imag:GoogleColab a imag:HostTypeEnumeration ;
    rdfs:label "Google Colab" .

imag:Grouping a imag:FeatureEnum ;
    rdfs:label "Grouping" ;
    skos:broader imag:Segmentation .

imag:HDF5 a imag:DatasetFormatEnumeration ;
    rdfs:label "HDF5 (Hierarchical Data Format)" .

imag:Icy a imag:IsPluginModuleOfEnum ;
    rdfs:label "icy" .

imag:IllustrativeImage a imag:ImageObjectTagEnum ;
    rdfs:label "illustrative image" .

imag:ImageEnhancement a imag:FeatureEnum ;
    rdfs:label "Image enhancement" ;
    skos:broader imag:Drawing .

imag:ImageQualityAssessment a imag:FeatureEnum ;
    rdfs:label "Image quality assessment" ;
    skos:broader imag:StatisticsMeasurement .

imag:ImageSimplification a imag:FeatureEnum ;
    rdfs:label "Image simplification" ;
    skos:broader imag:Preprocessing .

imag:InstanceSegmentation a imag:FeatureEnum ;
    rdfs:label "Instance segmentation" ;
    skos:broader imag:Segmentation .

imag:JPEG_PNG_TIFF a imag:DatasetFormatEnumeration ;
    rdfs:label "JPEG/PNG/TIFF (Standard Image Formats)" .

imag:JSON_XML a imag:DatasetFormatEnumeration ;
    rdfs:label "JSON/XML (Structured Data Formats)" .

imag:Java a imag:ComputerLanguageEnum ;
    rdfs:label "Java" .

imag:JavaScript a imag:ComputerLanguageEnum ;
    rdfs:label "JavaScript" .

imag:Labelling a imag:FeatureEnum ;
    rdfs:label "Labelling" ;
    skos:broader imag:Annotation .

imag:Library a imag:ApplicationCategoryEnum ;
    rdfs:label "Library" .

imag:Linux a imag:OperatingSystemEnum ;
    rdfs:label "Linux" .

imag:Logo a imag:ImageObjectTagEnum ;
    rdfs:label "logo" .

imag:MINC a imag:DatasetFormatEnumeration ;
    rdfs:label "MINC (Medical Imaging NetCDF)" .

imag:MRI a imag:ImagingModalityEnum ;
    rdfs:label "MRI" .

imag:MacOS a imag:OperatingSystemEnum ;
    rdfs:label "MacOS" .

imag:MatLab a imag:ComputerLanguageEnum ;
    rdfs:label "MATLAB" .

imag:ModelGeneration3d a imag:FeatureEnum ;
    rdfs:label "3d model generation" ;
    skos:broader imag:SceneReconstruction .

imag:MorphologicalReconstruction a imag:FeatureEnum ;
    rdfs:label "Morphological reconstruction" ;
    skos:broader imag:SceneReconstruction .

imag:MotionEstimation a imag:FeatureEnum ;
    rdfs:label "Motion estimation" ;
    skos:broader imag:OpticalFlow .

imag:NIfTI a imag:DatasetFormatEnumeration ;
    rdfs:label "NIfTI (Neuroimaging Informatics Technology Initiative)" .

imag:NRRD a imag:DatasetFormatEnumeration ;
    rdfs:label "NRRD (Nearly Raw Raster Data)" .

imag:Napari a imag:IsPluginModuleOfEnum ;
    rdfs:label "napari" .

imag:NoneAffiliation a imag:AffiliationEnum ;
    rdfs:label "None" .

imag:NonePluginModule a imag:IsPluginModuleOfEnum ;
    rdfs:label "None" .

imag:NoneProcessorRequirement a imag:ProcessorRequirementsEnum ;
    rdfs:label "None" .

imag:NoneSoftwareRequirement a imag:SoftwareRequirementsEnum ;
    rdfs:label "None" .

imag:Notebook a imag:ApplicationCategoryEnum ;
    rdfs:label "Notebook" .

imag:OMERO a imag:IsPluginModuleOfEnum ;
    rdfs:label "OMERO" .

imag:ObjectDetection a imag:FeatureEnum ;
    rdfs:label "Object detection" ;
    skos:broader imag:Segmentation .

imag:ObjectRecognition a imag:FeatureEnum ;
    rdfs:label "Object recognition" ;
    skos:broader imag:Segmentation .

imag:OrientationAnalysis a imag:FeatureEnum ;
    rdfs:label "Orientation analysis" ;
    skos:broader imag:PoseEstimation .

imag:OtherDatasetFormat a imag:DatasetFormatEnumeration ;
    rdfs:label "Other" .

imag:OtherHostType a imag:HostTypeEnumeration ;
    rdfs:label "Other" .

imag:OtherOS a imag:OperatingSystemEnum ;
    rdfs:label "Other" .

imag:Parquet a imag:DatasetFormatEnumeration ;
    rdfs:label "Parquet" .

imag:PatternRecognition a imag:FeatureEnum ;
    rdfs:label "Pattern recognition" ;
    skos:broader imag:Segmentation .

imag:PixelClassification a imag:FeatureEnum ;
    rdfs:label "Pixel classification" ;
    skos:broader imag:Segmentation .

imag:PlazaGradioApplication a imag:HostTypeEnumeration ;
    rdfs:label "Plaza Gradio Application" .

imag:Plugin a imag:ApplicationCategoryEnum ;
    rdfs:label "Plugin" .

imag:PoseDetection a imag:FeatureEnum ;
    rdfs:label "Pose detection" ;
    skos:broader imag:PoseEstimation .

imag:PoseInformation a imag:FeatureEnum ;
    rdfs:label "Pose information" ;
    skos:broader imag:PoseEstimation .

imag:PyTorch_1_13 a imag:SoftwareRequirementsEnum ;
    rdfs:label "PyTorch 1.13" .

imag:PyTorch_2_0 a imag:SoftwareRequirementsEnum ;
    rdfs:label "PyTorch 2.0" .

imag:PyTorch_2_1 a imag:SoftwareRequirementsEnum ;
    rdfs:label "PyTorch 2.1" .

imag:PyTorch_2_2 a imag:SoftwareRequirementsEnum ;
    rdfs:label "PyTorch 2.2" .

imag:Python a imag:ComputerLanguageEnum ;
    rdfs:label "Python" .

imag:Pyxu a imag:IsPluginModuleOfEnum ;
    rdfs:label "pyxu" .

imag:QuPath a imag:IsPluginModuleOfEnum ;
    rdfs:label "qupath" .

imag:QualityMetricMeasurement a imag:FeatureEnum ;
    rdfs:label "Quality metric measurement" ;
    skos:broader imag:StatisticsMeasurement .

imag:R a imag:ComputerLanguageEnum ;
    rdfs:label "R" .

imag:RAW a imag:DatasetFormatEnumeration ;
    rdfs:label "RAW (Unprocessed Binary Data)" .

imag:Reconstruction3d a imag:FeatureEnum ;
    rdfs:label "3d reconstruction" ;
    skos:broader imag:SceneReconstruction .

imag:Registration a imag:FeatureEnum ;
    rdfs:label "Registration" ;
    skos:broader imag:OpticalFlow .

imag:Rendering a imag:FeatureEnum ;
    rdfs:label "Rendering" ;
    skos:broader imag:Drawing .

imag:RenkuProject a imag:HostTypeEnumeration ;
    rdfs:label "Renku Project" .

imag:Rust a imag:ComputerLanguageEnum ;
    rdfs:label "Rust" .

imag:Scala a imag:ComputerLanguageEnum ;
    rdfs:label "Scala" .

imag:ShadingEstimation a imag:FeatureEnum ;
    rdfs:label "Shading estimation" ;
    skos:broader imag:SceneReconstruction .

imag:Shell a imag:ComputerLanguageEnum ;
    rdfs:label "shell" .

imag:Simulation a imag:FeatureEnum ;
    rdfs:label "Simulation" ;
    skos:broader imag:Modelling .

imag:Smoothing a imag:FeatureEnum ;
    rdfs:label "Smoothing" ;
    skos:broader imag:Denoising .

imag:Stitching a imag:FeatureEnum ;
    rdfs:label "Stitching" ;
    skos:broader imag:OpticalFlow .

imag:SurfaceParameterisation a imag:FeatureEnum ;
    rdfs:label "Surface parameterisation" ;
    skos:broader imag:MeshGeneration .

imag:TemplateMatching a imag:FeatureEnum ;
    rdfs:label "Template matching" ;
    skos:broader imag:Segmentation .

imag:Tensorflow_1_4 a imag:SoftwareRequirementsEnum ;
    rdfs:label "Tensorflow 1.4" .

imag:Tensorflow_1_5 a imag:SoftwareRequirementsEnum ;
    rdfs:label "Tensorflow 1.5" .

imag:Tensorflow_1_8 a imag:SoftwareRequirementsEnum ;
    rdfs:label "Tensorflow 1.8" .

imag:Tensorflow_2_0 a imag:SoftwareRequirementsEnum ;
    rdfs:label "Tensorflow 2.0" .

imag:Tensorflow_2_15 a imag:SoftwareRequirementsEnum ;
    rdfs:label "Tensorflow 2.15" .

imag:Tensorflow_2_2 a imag:SoftwareRequirementsEnum ;
    rdfs:label "Tensorflow 2.2" .

imag:Tensorflow_2_4 a imag:SoftwareRequirementsEnum ;
    rdfs:label "Tensorflow 2.4" .

imag:Tracking a imag:FeatureEnum ;
    rdfs:label "Tracking" .

imag:UNIL a imag:AffiliationEnum ;
    rdfs:label "UNIL" .

imag:UZH a imag:AffiliationEnum ;
    rdfs:label "UZH" .

imag:VisualQuestionAnswering a imag:FeatureEnum ;
    rdfs:label "Visual question answering" .

imag:Visualization a imag:FeatureEnum ;
    rdfs:label "Visualization" ;
    skos:broader imag:Drawing .

imag:Voxelization a imag:FeatureEnum ;
    rdfs:label "Voxelization" ;
    skos:broader imag:MeshGeneration .

imag:Wasm a imag:HostTypeEnumeration ;
    rdfs:label "WebAssembly" .

imag:WebApp a imag:ApplicationCategoryEnum ;
    rdfs:label "Web app" .

imag:Windows a imag:OperatingSystemEnum ;
    rdfs:label "Windows" .

imag:XRay a imag:ImagingModalityEnum ;
    rdfs:label "X-ray" .

sd:hasInput a rdf:Property ;
    rdfs:label "Has input"@en ;
    rdfs:comment "Property that links a model configuration to the input types expected by it."@en .

sd:hasOutput a rdf:Property ;
    rdfs:label "Has output"@en ;
    rdfs:comment "Property that expresses what the outputs of a model are"@en .

schema:CreativeWork-author a sh:PropertyShape ;
    sh:minCount 1 ;
    sh:or ( [ sh:class schema:Organization ] [ sh:class schema:Person ] ) ;
    sh:path schema:author .

schema:CreativeWork-citation a sh:PropertyShape ;
    sh:datatype xsd:string ;
    sh:minCount 1 ;
    sh:path schema:citation ;
    sh:pattern "^http.*" .

schema:CreativeWork-conditionsOfAccess a sh:PropertyShape ;
    sh:datatype xsd:string ;
    sh:path schema:conditionsOfAccess .

schema:CreativeWork-dateCreated a sh:PropertyShape ;
    sh:datatype xsd:date ;
    sh:maxCount 1 ;
    sh:minCount 1 ;
    sh:path schema:dateCreated .

schema:CreativeWork-datePublished a sh:PropertyShape ;
    sh:datatype xsd:date ;
    sh:minCount 1 ;
    sh:path schema:datePublished .

schema:CreativeWork-encodingFormat a sh:PropertyShape ;
    sh:path schema:encodingFormat ;
    sh:pattern ".*iana.org/assignments/media-types/.*" .

schema:CreativeWork-isAccessibleForFree a sh:PropertyShape ;
    sh:datatype xsd:boolean ;
    sh:path schema:isAccessibleForFree .

schema:CreativeWork-isBasedOn a sh:PropertyShape ;
    sh:path schema:isBasedOn ;
    sh:pattern "^http.*" .

schema:CreativeWork-keywords a sh:PropertyShape ;
    sh:datatype xsd:string ;
    sh:in ( "logo" "illustrative image" "before image" "after image" ) ;
    sh:maxCount 1 ;
    sh:minCount 1 ;
    sh:path schema:keywords .

schema:CreativeWork-license a sh:PropertyShape ;
    sh:minCount 1 ;
    sh:path schema:license ;
    sh:pattern ".*spdx\\.org.*" .

schema:DataDownload-contentURL a sh:PropertyShape ;
    sh:minCount 1 ;
    sh:path schema:contentUrl ;
    sh:pattern "^http.*" .

schema:Dataset-measurementTechnique a sh:PropertyShape ;
    sh:datatype xsd:string ;
    sh:path schema:measurementTechnique .

schema:Dataset-variableMeasured a sh:PropertyShape ;
    sh:datatype xsd:string ;
    sh:path schema:variableMeasured .

schema:ImageObject a sh:NodeShape ;
    sh:property schema:CreativeWork-keywords,
        schema:Thing-url .

schema:Organization-legalName a sh:PropertyShape ;
    sh:datatype xsd:string ;
    sh:minCount 1 ;
    sh:path schema:legalName .

schema:Person-affiliation a sh:PropertyShape ;
    sh:datatype xsd:string ;
    sh:path schema:affiliation .

schema:PropertyValueSpecification-defaultValue a sh:PropertyShape ;
    sh:datatype xsd:string ;
    sh:path schema:defaultValue .

schema:PropertyValueSpecification-valueRequired a sh:PropertyShape ;
    sh:datatype xsd:boolean ;
    sh:path schema:valueRequired .

schema:SoftwareApplication-applicationCategory a sh:PropertyShape ;
    sh:datatype xsd:string ;
    sh:path schema:applicationCategory .

schema:SoftwareApplication-featureList a sh:PropertyShape ;
    sh:datatype xsd:string ;
    sh:path schema:featureList .

schema:SoftwareApplication-memoryRequirements a sh:PropertyShape ;
    sh:or ( [ sh:datatype xsd:string ] [ sh:hasValue "None" ] ) ;
    sh:path schema:memoryRequirements .

schema:SoftwareApplication-operatingSystem a sh:PropertyShape ;
    sh:in ( "Linux" "Windows" "MacOS" "Other" ) ;
    sh:path schema:operatingSystem .

schema:SoftwareApplication-processorRequirements a sh:PropertyShape ;
    sh:datatype xsd:string ;
    sh:in ( "ARM64" "AMD64" "None" ) ;
    sh:path schema:processorRequirements .

schema:SoftwareApplication-softwareRequirements a sh:PropertyShape ;
    sh:datatype xsd:string ;
    sh:path schema:softwareRequirements .

schema:SoftwareApplication-softwareVersion a sh:PropertyShape ;
    sh:datatype xsd:string ;
    sh:minCount 1 ;
    sh:path schema:softwareVersion ;
    sh:pattern "[0-9]+\\.[0-9]+\\.[0-9]+" .

schema:SoftwareApplication-supportingData a sh:PropertyShape ;
    sh:class schema:DataFeed ;
    sh:path schema:supportingData .

schema:SoftwareSourceCode-codeRepository a sh:PropertyShape ;
    sh:maxCount 1 ;
    sh:minCount 1 ;
    sh:path schema:codeRepository ;
    sh:pattern "^http.*" .

schema:SoftwareSourceCode-programmingLanguage a sh:PropertyShape ;
    sh:datatype xsd:string ;
    sh:path schema:programmingLanguage .

schema:Thing-image a sh:PropertyShape ;
    sh:class schema:ImageObject ;
    sh:minCount 1 ;
    sh:path schema:image .

schema:affiliation a rdf:Property ;
    rdfs:label "Affiliation" ;
    rdfs:comment "An organization that this person is affiliated with. For example, a university (EPFL/ETHZ), lab, company." .

schema:applicationCategory a rdf:Property ;
    rdfs:label "Application category" ;
    rdfs:comment "Type of software application, e.g. 'Plugin, gui, desktop app, library'." .

schema:author a rdf:Property ;
    rdfs:label "Author" ;
    rdfs:comment "The author of the software, this can be organizations or people that are maintainers and/or producers of the software." .

schema:codeRepository a rdf:Property ;
    rdfs:label "Code repository" ;
    rdfs:comment "Primary link to the repository where the un-compiled, human readable code and related code is located (GitLab, GitHub, CodePlex etc.)." .

schema:conditionsOfAccess a rdf:Property ;
    rdfs:label "Conditions of access" ;
    rdfs:comment "Conditions that affect the availability of, or method(s) of access to, an item. e.g. log-in required " .

schema:contentUrl a rdf:Property ;
    rdfs:label "Content URL" ;
    rdfs:comment "Actual bytes of the media object, for example the image file or video file." .

schema:defaultValue a rdf:Property ;
    rdfs:label "Default value" ;
    rdfs:comment "The default value of the input. For properties that expect a literal, the default is a literal value, for properties that expect an object, it's an ID reference to one of the current values." .

schema:encodingFormat a rdf:Property ;
    rdfs:label "Encoding format" ;
    rdfs:comment "Expressed using a MIME format (http://www.iana.org/assignments/media-types/media-types.xhtml)." .

schema:familyName a rdf:Property ;
    rdfs:label "Family name" ;
    rdfs:comment "Family name. In the U.S., the last name of a Person." .

schema:givenName a rdf:Property ;
    rdfs:label "Given name" ;
    rdfs:comment "Given name. In the U.S., the first name of a Person." .

schema:identifier a rdf:Property ;
    rdfs:label "Identifier" ;
    rdfs:comment "Represents any kind of unique string to identify something, such as ISBNs, GTIN codes, UUIDs etc." .

schema:isAccessibleForFree a rdf:Property ;
    rdfs:label "Is accessible for free" ;
    rdfs:comment "A flag to signal that the item, event, or place is accessible for free." .

schema:isBasedOn a rdf:Property ;
    rdfs:label "Is based on" ;
    rdfs:comment "A resource from which this work is derived or from which it is a modification or adaption." .

schema:keywords a rdf:Property ;
    rdfs:label "Keywords"@en ;
    rdfs:comment "The keywords/tags used to describe this content."@en .

schema:legalName a rdf:Property ;
    rdfs:label "Legal name" ;
    rdfs:comment "The official name of the organization, e.g. the registered company name." .

schema:measurementTechnique a rdf:Property ;
    rdfs:label "Measurement technique" ;
    rdfs:comment "A technique or technology used in a Dataset corresponding to the method used for measuring the corresponding variable(s)." .

schema:name a rdf:Property ;
    rdfs:label "Name" ;
    rdfs:comment "The name of a person, in the US their first and last name(s) seperated by spaces" .

schema:operatingSystem a rdf:Property ;
    rdfs:label "Operating system" ;
    rdfs:comment "Operating systems supported (Windows 7/10/11, OS X 10.6, Android 1.6)." .

schema:processorRequirements a rdf:Property ;
    rdfs:label "Processor requirements" ;
    rdfs:comment "Processor architecture required to run the application." .

schema:softwareVersion a rdf:Property ;
    rdfs:label "Software version" ;
    rdfs:comment "Version of the software instance." .

schema:valueRequired a rdf:Property ;
    rdfs:label "Value required" ;
    rdfs:comment "Whether the property must be filled in to complete the action. Default is false." .

schema:variableMeasured a rdf:Property ;
    rdfs:label "Variable measured" ;
    rdfs:comment "The variables that are measured in some dataset, described as text." .

md4i:hasRorId a rdf:Property ;
    rdfs:label "Has ROR ID" ;
    rdfs:comment "A Research Organization Registry identifier, that points to a research organization" .

md4i:hasRorIdShape a sh:PropertyShape ;
    sh:path md4i:hasRorId ;
    sh:pattern "^http.*" .

md4i:orcidId a rdf:Property ;
    rdfs:label "Has ORCID ID" ;
    rdfs:comment "The ORCID ID of a person" .

md4i:orcidIdShape a sh:PropertyShape ;
    sh:datatype xsd:string ;
    sh:path md4i:orcidId .

dmib:hasPhysicalQuantity a rdf:Property ;
    rdfs:label "Has physical quantity"@en ;
    rdfs:comment "Property to indicate the physical quantity of the input or output of a dataset specification"@en .

sphn:bodySite a rdf:Property ;
    rdfs:label "Body site"@en ;
    rdfs:comment "The part of the body that is being imaged."@en .

imag: a owl:Ontology ;
    dcterms:abstract "The Imaging Plaza ontology provides concepts (classes and properties) to model human and machine readable imaging software metadata. It is the result of re-using external pre-existing vocabularies such as schema.org and the software description ontology, together with custom imaging specific objects and properties." ;
    dcterms:contributor "Carlos Vivar Rios",
        "Robin Franken" ;
    dcterms:created "2024-04-01"^^xsd:date ;
    dcterms:creator "Robin Franken" ;
    dcterms:description "The Imaging Plaza ontology provides concepts (classes and properties) to model human and machine readable imaging software metadata. It is the result of re-using external pre-existing vocabularies such as schema.org and the software description ontology, together with custom imaging specific objects and properties. The ontology contains purely semantic information (labels, definitions etc.) and is meant to be used in conjuction with a graph of enumeration values and a graph containing SHACL shapes to provide more machine readable restrictions on values of properties." ;
    dcterms:license <https://spdx.org/licenses/CC-BY-SA-4.0.html> ;
    dcterms:modified "2025-01-28"^^xsd:date ;
    dcterms:title "Imaging Plaza Ontology" ;
    vann:preferredNamespacePrefix "imag" ;
    vann:preferredNamespaceUri "https://imaging-plaza.epfl.ch/ontology#"^^xsd:string ;
    owl:versionInfo "0.8.0"^^xsd:string ;
    sh:declare [ sh:namespace imag: ;
            sh:prefix "imag" ] ;
    sh:entailment sh:Rules .

imag:Annotation a imag:FeatureEnum ;
    rdfs:label "Annotation" .

imag:FeatureTaggerRule a sh:SPARQLRule ;
    sh:construct """
    PREFIX rdfs: <http://www.w3.org/2000/01/rdf-schema#>
    PREFIX schema: <http://schema.org/>
    PREFIX skos: <http://www.w3.org/2004/02/skos/core#>
			CONSTRUCT {
				$this schema:featureList ?parentFeatureLabel .
                $this schema:featureList ?feature .
			}
			WHERE {
				$this schema:featureList ?feature .
                ?featureClass rdfs:label ?feature .
				?featureClass skos:broader ?parentFeature.
                ?parentFeature rdfs:label ?parentFeatureLabel .
			}
			""" ;
    sh:description "This shape is used to extend the initial tagging of a software with it's higher level tags, for ease of retrieval/filtering" ;
    sh:name "Feature tagger" .

imag:Modelling a imag:FeatureEnum ;
    rdfs:label "Modelling" .

imag:MorphologicalAnalysis a imag:FeatureEnum ;
    rdfs:label "Morphological analysis" .

imag:SoftwareApplication-hasExecutableNotebook a sh:PropertyShape ;
    sh:class imag:ExecutableNotebook ;
    sh:path imag:hasExecutableNotebook .

imag:SoftwareApplication-requiresGPUShape a sh:PropertyShape ;
    sh:datatype xsd:boolean ;
    sh:path imag:requiresGPU .

imag:SoftwareApplication-runnableExampleShape a sh:PropertyShape ;
    sh:class imag:RunnableExample ;
    sh:path imag:runnableExample .

imag:bodySiteShape a sh:PropertyShape ;
    sh:datatype xsd:string ;
    sh:path sphn:bodySite .

imag:datasetFormat a rdf:Property ;
    rdfs:label "Dataset format"@en ;
    rdfs:comment "The format of the dataset. For example, dicom, nifti, tiff, png, jpg, etc."@en .

imag:datasetFormatShape a sh:PropertyShape ;
    sh:datatype xsd:string ;
    sh:in ( "DICOM (Digital Imaging and Communications in Medicine)" "NIfTI (Neuroimaging Informatics Technology Initiative)" "MINC (Medical Imaging NetCDF)" "NRRD (Nearly Raw Raster Data)" "HDF5 (Hierarchical Data Format)" "Parquet" "CSV/TSV (Tabular Data)" "JSON/XML (Structured Data Formats)" "JPEG/PNG/TIFF (Standard Image Formats)" "RAW (Unprocessed Binary Data)" "Other" ) ;
    sh:path imag:datasetFormat .

imag:fairLevelShape a sh:PropertyShape ;
    sh:datatype xsd:string ;
    sh:minCount 1 ;
    sh:path imag:fairLevel .

imag:fairlevel0Shape a sh:NodeShape .

imag:fairlevel5Shape a sh:NodeShape ;
    sh:and ( imag:fairlevel4Shape ) ;
    sh:property [ sh:message "Fair level 5" ;
            sh:minCount 1 ;
            sh:path sd:hasExecutableInstructions ] ;
    sh:targetClass schema:SoftwareSourceCode .

imag:hasExecutableNotebook a rdf:Property ;
    rdfs:label "Has executable notebook"@en ;
    rdfs:comment "Property that links a software component with an executable notebook (e.g., Jupyter notebook)."@en .

imag:hasPhysicalQuantityShape a sh:PropertyShape ;
    sh:datatype xsd:string ;
    sh:path dmib:hasPhysicalQuantity .

imag:hostType a rdf:Property ;
    rdfs:label "Host type"@en ;
    rdfs:comment "The type of host that the software component is running on. For example, plaza-gradio-application, renku-project, google-colab, wasm, other"@en .

imag:hostTypeShape a sh:PropertyShape ;
    sh:datatype xsd:string ;
    sh:in ( "plaza-gradio-application" "renku-project" "google-colab" "wasm" "other" ) ;
    sh:path imag:hostType .

imag:imagingModality a rdf:Property ;
    rdfs:label "Imaging modality" ;
    rdfs:comment "Technique or method used to create images of the interior of a body or an object for which this software was designed." .

imag:isPluginModuleOf a rdf:Property ;
    rdfs:label "Is plugin/module of" ;
    rdfs:comment "The resource for which this tool is a plugin or module." .

imag:isPluginModuleOfShape a sh:PropertyShape ;
    sh:datatype xsd:string ;
    sh:path imag:isPluginModuleOf .

imag:relatedToOrganization a rdf:Property ;
    rdfs:label "Related to organization" ;
    rdfs:comment "The lab/institution/group/project/organization to which a software is related and/or affiliated to" .

imag:relatedToOrganizationShape a sh:PropertyShape ;
    sh:datatype xsd:string ;
    sh:path imag:relatedToOrganization .

imag:requiresGPU a rdf:Property ;
    rdfs:label "Requires GPU" ;
    rdfs:comment "Stipulates whether something requires a graphical processing unit such as a NVIDEA or AMD graphics card" .

imag:resolution a rdf:Property ;
    rdfs:label "Resolution" ;
    rdfs:comment "The resolution of the image." .

imag:resolutionShape a sh:PropertyShape ;
    sh:datatype xsd:string ;
    sh:path imag:resolution .

imag:runnableExample a rdf:Property ;
    rdfs:label "Runnable example" ;
    rdfs:comment "A runnable example of the software component"@en .

sd:DatasetSpecification-hasFormat a sh:PropertyShape ;
    sh:datatype xsd:string ;
    sh:path sd:hasFormat .

sd:FundingInformation-fundingGrant a sh:PropertyShape ;
    sh:datatype xsd:string ;
    sh:minCount 1 ;
    sh:path sd:fundingGrant .

sd:FundingInformation-fundingSource a sh:PropertyShape ;
    sh:class schema:Organization ;
    sh:minCount 1 ;
    sh:path sd:fundingSource .

sd:SoftwareApplication-hasAcknowledgements a sh:PropertyShape ;
    sh:datatype xsd:string ;
    sh:path sd:hasAcknowledgements .

sd:SoftwareApplication-hasDocumentation a sh:PropertyShape ;
    sh:path sd:hasDocumentation ;
    sh:pattern "^http.*" .

sd:SoftwareApplication-hasExecutableInstructions a sh:PropertyShape ;
    sh:datatype xsd:string ;
    sh:path sd:hasExecutableInstructions .

sd:SoftwareApplication-hasFunding a sh:PropertyShape ;
    sh:class sd:FundingInformation ;
    sh:path sd:hasFunding .

sd:SoftwareApplication-hasParameter a sh:PropertyShape ;
    sh:class bio:FormalParameter ;
    sh:path sd:hasParameter .

sd:SoftwareApplication-readme a sh:PropertyShape ;
    sh:path sd:readme ;
    sh:pattern "^http.*" .

sd:SoftwareConfiguration-hasSoftwareImage a sh:PropertyShape ;
    sh:class sd:SoftwareImage ;
    sh:path sd:hasSoftwareImage .

sd:SoftwareImage-availableInRegistry a sh:PropertyShape ;
    sh:path sd:availableInRegistry ;
    sh:pattern "^http.*" .

sd:availableInRegistry a rdf:Property ;
    rdfs:label "Available in registry"@en ;
    rdfs:comment "URL to registry of where software image can be found. For example, https://hub.docker.com/r/pytorch/pytorch"@en .

sd:fundingGrant a rdf:Property ;
    rdfs:label "Funding grant"@en ;
    rdfs:comment "Grant number used for funding"@en ;
    rdfs:subPropertyOf <https://codemeta.github.io/terms/funding> .

sd:fundingSource a rdf:Property ;
    rdfs:label "Funding source"@en ;
    rdfs:comment "Link to an organization funding a software/component"@en ;
    rdfs:subPropertyOf owl:topObjectProperty .

sd:hasAcknowledgements a rdf:Property ;
    rdfs:label "Has acknowledgements"@en ;
    rdfs:comment "String with the people, organizations and other contributors acknowledged by the authors."@en .

sd:hasDimensionality a rdf:Property ;
    rdfs:label "Has dimensionality"@en ;
    rdfs:comment "Property to indicate dimensionality of the input or output of a dataset specification"@en .

sd:hasFormat a rdf:Property ;
    rdfs:label "Has format"@en ;
    rdfs:comment "Format followed by a file. For example, txt, nc, etc."@en .

sd:hasFunding a rdf:Property ;
    rdfs:label "Has funding information"@en ;
    rdfs:comment "Property that links a software project to its funding information"@en .

sd:hasParameter a rdf:Property ;
    rdfs:label "Has parameter"@en ;
    rdfs:comment "Property that indicates the parameters of a model configuration"@en .

schema:Thing-identifier a sh:PropertyShape ;
    sh:datatype xsd:string ;
    sh:minCount 1 ;
    sh:path schema:identifier .

schema:citation a rdf:Property ;
    rdfs:label "Citation DOI" ;
    rdfs:comment "A DOI https URL citation to publication about this software. Use Zenodo to generate if needed. e.g. https://doi.org/10.1016/j.procs.2017.03.009" .

schema:dateCreated a rdf:Property ;
    rdfs:label "Date created" ;
    rdfs:comment "The date on which the repository was created." .

schema:datePublished a rdf:Property ;
    rdfs:label "Date published" ;
    rdfs:comment "Latest published git release date, else, the publish date of the doi." .

schema:description a rdf:Property ;
    rdfs:label "Description" ;
    rdfs:comment "A description of the item." .

schema:featureList a rdf:Property ;
    rdfs:label "Feature list" ;
    rdfs:comment "Features or modules provided by this application (and possibly required by other applications)." .

schema:image a rdf:Property ;
    rdfs:label "Image" ;
    rdfs:comment "An image of the item." .

schema:license a rdf:Property ;
    rdfs:label "License" ;
    rdfs:comment "A license document that applies to this content, typically indicated by URL." .

schema:memoryRequirements a rdf:Property ;
    rdfs:label "Memory requirements" ;
    rdfs:comment "Minimum RAM requirements in GB to run the software, 0 if not applicable." .

schema:programmingLanguage a rdf:Property ;
    rdfs:label "Programming Language" ;
    rdfs:comment "The computer programming language." .

schema:softwareRequirements a rdf:Property ;
    rdfs:label "Software requirements" ;
    rdfs:comment "Special third party dependencies (e.g. CUDA, Tensorflow etc. related requirements)." .

schema:supportingData a rdf:Property ;
    rdfs:label "Supporting data" ;
    rdfs:comment "Supporting data for a SoftwareApplication." .

schema:url a rdf:Property ;
    rdfs:label "URL" ;
    rdfs:comment "Fill in any URL related to this repository. e.g. related lab or project website." .

imag:FeatureExtraction a imag:FeatureEnum ;
    rdfs:label "Feature extraction" .

imag:MeshGeneration a imag:FeatureEnum ;
    rdfs:label "Mesh generation" .

imag:Preprocessing a imag:FeatureEnum ;
    rdfs:label "Preprocessing" .

imag:SoftwareApplication-imagingModalityShape a sh:PropertyShape ;
    sh:datatype xsd:string ;
    sh:path imag:imagingModality .

imag:fairlevel1Shape a sh:NodeShape ;
    sh:property [ sh:message "Fair level 1" ;
            sh:minCount 1 ;
            sh:path schema:license ],
        [ sh:message "Fair level 1" ;
            sh:minCount 1 ;
            sh:path schema:citation ],
        [ sh:message "Fair level 1" ;
            sh:minCount 1 ;
            sh:path schema:description ],
        [ sh:message "Fair level 1" ;
            sh:minCount 1 ;
            sh:path schema:url ],
        [ sh:message "Fair level 1" ;
            sh:minCount 1 ;
            sh:path schema:dateCreated ],
        [ sh:message "Fair level 1" ;
            sh:minCount 1 ;
            sh:path schema:datePublished ],
        [ sh:message "Fair level 1" ;
            sh:minCount 1 ;
            sh:path schema:image ] ;
    sh:targetClass schema:SoftwareSourceCode .

imag:fairlevel2Shape a sh:NodeShape ;
    sh:and ( imag:fairlevel1Shape ) ;
    sh:property [ sh:message "Fair level 2" ;
            sh:minCount 1 ;
            sh:path schema:programmingLanguage ],
        [ sh:message "Fair level 2" ;
            sh:minCount 1 ;
            sh:path schema:featureList ],
        [ sh:message "Fair level 2" ;
            sh:minCount 1 ;
            sh:path sd:readme ] ;
    sh:targetClass schema:SoftwareSourceCode .

imag:fairlevel3Shape a sh:NodeShape ;
    sh:and ( imag:fairlevel2Shape ) ;
    sh:property [ sh:message "Fair level 3" ;
            sh:minCount 1 ;
            sh:path schema:softwareRequirements ],
        [ sh:message "Fair level 3" ;
            sh:minCount 1 ;
            sh:path schema:supportingData ] ;
    sh:targetClass schema:SoftwareSourceCode .

imag:fairlevel4Shape a sh:NodeShape ;
    sh:and ( imag:fairlevel3Shape ) ;
    sh:property [ sh:message "Fair level 4" ;
            sh:minCount 1 ;
            sh:path schema:memoryRequirements ],
        [ sh:message "Fair level 4" ;
            sh:minCount 1 ;
            sh:path sd:hasDocumentation ],
        [ sh:message "Fair level 4" ;
            sh:minCount 1 ;
            sh:path sd:hasSoftwareImage ] ;
    sh:targetClass schema:SoftwareSourceCode .

sd:DatasetSpecification-hasDimensionality a sh:PropertyShape ;
    sh:datatype xsd:integer ;
    sh:minExclusive 0 ;
    sh:path sd:hasDimensionality .

sd:hasDocumentation a rdf:Property ;
    rdfs:label "Has documentation"@en ;
    rdfs:comment "Pointer to the documentation of the model"@en .

sd:hasExecutableInstructions a rdf:Property ;
    rdfs:label "Has executable instructions"@en ;
    rdfs:comment "URL to Human-readable instructions that indicate how a software component should be executed."@en .

sd:hasSoftwareImage a rdf:Property ;
    rdfs:label "Has software image"@en ;
    rdfs:comment "Function to link a function with its corresponding container"@en .

sd:readme a rdf:Property ;
    rdfs:label "Readme"@en ;
    rdfs:comment "URL to the Readme file of a software component"@en ;
    rdfs:subPropertyOf <https://codemeta.github.io/terms/readme> .

imag:Denoising a imag:FeatureEnum ;
    rdfs:label "Denoising" .

imag:Drawing a imag:FeatureEnum ;
    rdfs:label "Drawing" .

imag:PoseEstimation a imag:FeatureEnum ;
    rdfs:label "Pose estimation" .

imag:StatisticsMeasurement a imag:FeatureEnum ;
    rdfs:label "Statistics measurement" .

schema:Thing-url a sh:PropertyShape ;
    sh:path schema:url ;
    sh:pattern "^http.*" .

imag:OpticalFlow a imag:FeatureEnum ;
    rdfs:label "Optical flow" .

schema:Thing-description a sh:PropertyShape ;
    sh:datatype xsd:string ;
    sh:maxLength 2000 ;
    sh:minCount 1 ;
    sh:path schema:description .

imag:SceneReconstruction a imag:FeatureEnum ;
    rdfs:label "Scene reconstruction" .

schema:Thing-name a sh:PropertyShape ;
    sh:datatype xsd:string ;
    sh:maxLength 60 ;
    sh:minCount 1 ;
    sh:path schema:name .

imag:fairLevel a rdf:Property ;
    rdfs:label "FAIR Level" ;
    rdfs:comment "A score of 1-5 rating the Findability, Accessibility, Interoperability and Reusability of a piece of software based on the presence of certain properties for an instance of software" .

imag:Segmentation a imag:FeatureEnum ;
    rdfs:label "Segmentation" .

